refactor: rename normalOrder for CrAnAlgebra

HepLean/PerturbationTheory/Algebras/CrAnAlgebra/NormalOrder.lean
@@ -32,24 +32,24 @@ noncomputable section
   a list of CrAnStates to the normal-ordered list of states multiplied by
   the sign corresponding to the number of fermionic-fermionic
   exchanges done in ordering. -/
-def normalOrder : CrAnAlgebra 𝓕 →ₗ[ℂ] CrAnAlgebra 𝓕 :=
+def normalOrderF : CrAnAlgebra 𝓕 →ₗ[ℂ] CrAnAlgebra 𝓕 :=
   Basis.constr ofCrAnListBasis ℂ fun φs =>
   normalOrderSign φs • ofCrAnList (normalOrderList φs)
 
-@[inherit_doc normalOrder]
-scoped[FieldSpecification.CrAnAlgebra] notation "𝓝ᶠ(" a ")" => normalOrder a
+@[inherit_doc normalOrderF]
+scoped[FieldSpecification.CrAnAlgebra] notation "𝓝ᶠ(" a ")" => normalOrderF a
 
-lemma normalOrder_ofCrAnList (φs : List 𝓕.CrAnStates) :
+lemma normalOrderF_ofCrAnList (φs : List 𝓕.CrAnStates) :
     𝓝ᶠ(ofCrAnList φs) = normalOrderSign φs • ofCrAnList (normalOrderList φs) := by
-  rw [← ofListBasis_eq_ofList, normalOrder, Basis.constr_basis]
+  rw [← ofListBasis_eq_ofList, normalOrderF, Basis.constr_basis]
 
-lemma ofCrAnList_eq_normalOrder (φs : List 𝓕.CrAnStates) :
+lemma ofCrAnList_eq_normalOrderF (φs : List 𝓕.CrAnStates) :
     ofCrAnList (normalOrderList φs) = normalOrderSign φs • 𝓝ᶠ(ofCrAnList φs) := by
-  rw [normalOrder_ofCrAnList, normalOrderList, smul_smul, normalOrderSign, Wick.koszulSign_mul_self,
+  rw [normalOrderF_ofCrAnList, normalOrderList, smul_smul, normalOrderSign, Wick.koszulSign_mul_self,
     one_smul]
 
-lemma normalOrder_one : normalOrder (𝓕 := 𝓕) 1 = 1 := by
-  rw [← ofCrAnList_nil, normalOrder_ofCrAnList, normalOrderSign_nil, normalOrderList_nil,
+lemma normalOrderF_one : normalOrderF (𝓕 := 𝓕) 1 = 1 := by
+  rw [← ofCrAnList_nil, normalOrderF_ofCrAnList, normalOrderSign_nil, normalOrderList_nil,
     ofCrAnList_nil, one_smul]
 
 /-!
@@ -58,130 +58,130 @@ lemma normalOrder_one : normalOrder (𝓕 := 𝓕) 1 = 1 := by
 
 -/
 
-lemma normalOrder_ofCrAnList_cons_create (φ : 𝓕.CrAnStates)
+lemma normalOrderF_ofCrAnList_cons_create (φ : 𝓕.CrAnStates)
     (hφ : 𝓕 |>ᶜ φ = CreateAnnihilate.create) (φs : List 𝓕.CrAnStates) :
     𝓝ᶠ(ofCrAnList (φ :: φs)) = ofCrAnState φ * 𝓝ᶠ(ofCrAnList φs) := by
-  rw [normalOrder_ofCrAnList, normalOrderSign_cons_create φ hφ, normalOrderList_cons_create φ hφ φs]
-  rw [ofCrAnList_cons, normalOrder_ofCrAnList, mul_smul_comm]
+  rw [normalOrderF_ofCrAnList, normalOrderSign_cons_create φ hφ, normalOrderList_cons_create φ hφ φs]
+  rw [ofCrAnList_cons, normalOrderF_ofCrAnList, mul_smul_comm]
 
-lemma normalOrder_create_mul (φ : 𝓕.CrAnStates)
+lemma normalOrderF_create_mul (φ : 𝓕.CrAnStates)
     (hφ : 𝓕 |>ᶜ φ = CreateAnnihilate.create) (a : CrAnAlgebra 𝓕) :
     𝓝ᶠ(ofCrAnState φ * a) = ofCrAnState φ * 𝓝ᶠ(a) := by
-  change (normalOrder ∘ₗ mulLinearMap (ofCrAnState φ)) a =
-    (mulLinearMap (ofCrAnState φ) ∘ₗ normalOrder) a
+  change (normalOrderF ∘ₗ mulLinearMap (ofCrAnState φ)) a =
+    (mulLinearMap (ofCrAnState φ) ∘ₗ normalOrderF) a
   refine LinearMap.congr_fun (ofCrAnListBasis.ext fun l ↦ ?_) a
   simp only [mulLinearMap, LinearMap.coe_mk, AddHom.coe_mk, ofListBasis_eq_ofList,
     LinearMap.coe_comp, Function.comp_apply]
-  rw [← ofCrAnList_cons, normalOrder_ofCrAnList_cons_create φ hφ]
+  rw [← ofCrAnList_cons, normalOrderF_ofCrAnList_cons_create φ hφ]
 
-lemma normalOrder_ofCrAnList_append_annihilate (φ : 𝓕.CrAnStates)
+lemma normalOrderF_ofCrAnList_append_annihilate (φ : 𝓕.CrAnStates)
     (hφ : 𝓕 |>ᶜ φ = CreateAnnihilate.annihilate) (φs : List 𝓕.CrAnStates) :
     𝓝ᶠ(ofCrAnList (φs ++ [φ])) = 𝓝ᶠ(ofCrAnList φs) * ofCrAnState φ := by
-  rw [normalOrder_ofCrAnList, normalOrderSign_append_annihlate φ hφ φs,
+  rw [normalOrderF_ofCrAnList, normalOrderSign_append_annihlate φ hφ φs,
     normalOrderList_append_annihilate φ hφ φs, ofCrAnList_append, ofCrAnList_singleton,
-      normalOrder_ofCrAnList, smul_mul_assoc]
+      normalOrderF_ofCrAnList, smul_mul_assoc]
 
-lemma normalOrder_mul_annihilate (φ : 𝓕.CrAnStates)
+lemma normalOrderF_mul_annihilate (φ : 𝓕.CrAnStates)
     (hφ : 𝓕 |>ᶜ φ = CreateAnnihilate.annihilate)
     (a : CrAnAlgebra 𝓕) : 𝓝ᶠ(a * ofCrAnState φ) = 𝓝ᶠ(a) * ofCrAnState φ := by
-  change (normalOrder ∘ₗ mulLinearMap.flip (ofCrAnState φ)) a =
-    (mulLinearMap.flip (ofCrAnState φ) ∘ₗ normalOrder) a
+  change (normalOrderF ∘ₗ mulLinearMap.flip (ofCrAnState φ)) a =
+    (mulLinearMap.flip (ofCrAnState φ) ∘ₗ normalOrderF) a
   refine LinearMap.congr_fun (ofCrAnListBasis.ext fun l ↦ ?_) a
   simp only [mulLinearMap, ofListBasis_eq_ofList, LinearMap.coe_comp, Function.comp_apply,
     LinearMap.flip_apply, LinearMap.coe_mk, AddHom.coe_mk]
   rw [← ofCrAnList_singleton, ← ofCrAnList_append, ofCrAnList_singleton,
-    normalOrder_ofCrAnList_append_annihilate φ hφ]
+    normalOrderF_ofCrAnList_append_annihilate φ hφ]
 
-lemma normalOrder_crPart_mul (φ : 𝓕.States) (a : CrAnAlgebra 𝓕) :
+lemma normalOrderF_crPart_mul (φ : 𝓕.States) (a : CrAnAlgebra 𝓕) :
     𝓝ᶠ(crPart φ * a) =
     crPart φ * 𝓝ᶠ(a) := by
   match φ with
   | .inAsymp φ =>
     rw [crPart]
-    exact normalOrder_create_mul ⟨States.inAsymp φ, ()⟩ rfl a
+    exact normalOrderF_create_mul ⟨States.inAsymp φ, ()⟩ rfl a
   | .position φ =>
     rw [crPart]
-    exact normalOrder_create_mul _ rfl _
+    exact normalOrderF_create_mul _ rfl _
   | .outAsymp φ => simp
 
-lemma normalOrder_mul_anPart (φ : 𝓕.States) (a : CrAnAlgebra 𝓕) :
+lemma normalOrderF_mul_anPart (φ : 𝓕.States) (a : CrAnAlgebra 𝓕) :
     𝓝ᶠ(a * anPart φ) =
     𝓝ᶠ(a) * anPart φ := by
   match φ with
   | .inAsymp φ => simp
   | .position φ =>
     rw [anPart]
-    exact normalOrder_mul_annihilate _ rfl _
+    exact normalOrderF_mul_annihilate _ rfl _
   | .outAsymp φ =>
     rw [anPart]
-    refine normalOrder_mul_annihilate _ rfl _
+    refine normalOrderF_mul_annihilate _ rfl _
 
 /-!
 
 ## Normal ordering for an adjacent creation and annihliation state
 
-The main result of this section is `normalOrder_superCommuteF_annihilate_create`.
+The main result of this section is `normalOrderF_superCommuteF_annihilate_create`.
 -/
 
-lemma normalOrder_swap_create_annihlate_ofCrAnList_ofCrAnList (φc φa : 𝓕.CrAnStates)
+lemma normalOrderF_swap_create_annihlate_ofCrAnList_ofCrAnList (φc φa : 𝓕.CrAnStates)
     (hφc : 𝓕 |>ᶜ φc = CreateAnnihilate.create) (hφa : 𝓕 |>ᶜ φa = CreateAnnihilate.annihilate)
     (φs φs' : List 𝓕.CrAnStates) :
     𝓝ᶠ(ofCrAnList φs' * ofCrAnState φc * ofCrAnState φa * ofCrAnList φs) = 𝓢(𝓕 |>ₛ φc, 𝓕 |>ₛ φa) •
     𝓝ᶠ(ofCrAnList φs' * ofCrAnState φa * ofCrAnState φc * ofCrAnList φs) := by
   rw [mul_assoc, mul_assoc, ← ofCrAnList_cons, ← ofCrAnList_cons, ← ofCrAnList_append]
-  rw [normalOrder_ofCrAnList, normalOrderSign_swap_create_annihlate φc φa hφc hφa]
-  rw [normalOrderList_swap_create_annihlate φc φa hφc hφa, ← smul_smul, ← normalOrder_ofCrAnList]
+  rw [normalOrderF_ofCrAnList, normalOrderSign_swap_create_annihlate φc φa hφc hφa]
+  rw [normalOrderList_swap_create_annihlate φc φa hφc hφa, ← smul_smul, ← normalOrderF_ofCrAnList]
   rw [ofCrAnList_append, ofCrAnList_cons, ofCrAnList_cons]
   noncomm_ring
 
-lemma normalOrder_swap_create_annihlate_ofCrAnList (φc φa : 𝓕.CrAnStates)
+lemma normalOrderF_swap_create_annihlate_ofCrAnList (φc φa : 𝓕.CrAnStates)
     (hφc : 𝓕 |>ᶜ φc = CreateAnnihilate.create) (hφa : 𝓕 |>ᶜ φa = CreateAnnihilate.annihilate)
     (φs : List 𝓕.CrAnStates) (a : 𝓕.CrAnAlgebra) :
     𝓝ᶠ(ofCrAnList φs * ofCrAnState φc * ofCrAnState φa * a) = 𝓢(𝓕 |>ₛ φc, 𝓕 |>ₛ φa) •
     𝓝ᶠ(ofCrAnList φs * ofCrAnState φa * ofCrAnState φc * a) := by
-  change (normalOrder ∘ₗ mulLinearMap (ofCrAnList φs * ofCrAnState φc * ofCrAnState φa)) a =
-    (smulLinearMap _ ∘ₗ normalOrder ∘ₗ
+  change (normalOrderF ∘ₗ mulLinearMap (ofCrAnList φs * ofCrAnState φc * ofCrAnState φa)) a =
+    (smulLinearMap _ ∘ₗ normalOrderF ∘ₗ
     mulLinearMap (ofCrAnList φs * ofCrAnState φa * ofCrAnState φc)) a
   refine LinearMap.congr_fun (ofCrAnListBasis.ext fun l ↦ ?_) a
   simp only [mulLinearMap, LinearMap.coe_mk, AddHom.coe_mk, ofListBasis_eq_ofList,
     LinearMap.coe_comp, Function.comp_apply, instCommGroup.eq_1]
-  rw [normalOrder_swap_create_annihlate_ofCrAnList_ofCrAnList φc φa hφc hφa]
+  rw [normalOrderF_swap_create_annihlate_ofCrAnList_ofCrAnList φc φa hφc hφa]
   rfl
 
-lemma normalOrder_swap_create_annihlate (φc φa : 𝓕.CrAnStates)
+lemma normalOrderF_swap_create_annihlate (φc φa : 𝓕.CrAnStates)
     (hφc : 𝓕 |>ᶜ φc = CreateAnnihilate.create) (hφa : 𝓕 |>ᶜ φa = CreateAnnihilate.annihilate)
     (a b : 𝓕.CrAnAlgebra) :
     𝓝ᶠ(a * ofCrAnState φc * ofCrAnState φa * b) = 𝓢(𝓕 |>ₛ φc, 𝓕 |>ₛ φa) •
     𝓝ᶠ(a * ofCrAnState φa * ofCrAnState φc * b) := by
   rw [mul_assoc, mul_assoc, mul_assoc, mul_assoc]
-  change (normalOrder ∘ₗ mulLinearMap.flip (ofCrAnState φc * (ofCrAnState φa * b))) a =
+  change (normalOrderF ∘ₗ mulLinearMap.flip (ofCrAnState φc * (ofCrAnState φa * b))) a =
     (smulLinearMap (𝓢(𝓕 |>ₛ φc, 𝓕 |>ₛ φa)) ∘ₗ
-    normalOrder ∘ₗ mulLinearMap.flip (ofCrAnState φa * (ofCrAnState φc * b))) a
+    normalOrderF ∘ₗ mulLinearMap.flip (ofCrAnState φa * (ofCrAnState φc * b))) a
   refine LinearMap.congr_fun (ofCrAnListBasis.ext fun l ↦ ?_) _
   simp only [mulLinearMap, ofListBasis_eq_ofList, LinearMap.coe_comp, Function.comp_apply,
     LinearMap.flip_apply, LinearMap.coe_mk, AddHom.coe_mk, instCommGroup.eq_1, ← mul_assoc,
-      normalOrder_swap_create_annihlate_ofCrAnList φc φa hφc hφa]
+      normalOrderF_swap_create_annihlate_ofCrAnList φc φa hφc hφa]
   rfl
 
-lemma normalOrder_superCommuteF_create_annihilate (φc φa : 𝓕.CrAnStates)
+lemma normalOrderF_superCommuteF_create_annihilate (φc φa : 𝓕.CrAnStates)
     (hφc : 𝓕 |>ᶜ φc = CreateAnnihilate.create) (hφa : 𝓕 |>ᶜ φa = CreateAnnihilate.annihilate)
     (a b : 𝓕.CrAnAlgebra) :
     𝓝ᶠ(a * [ofCrAnState φc, ofCrAnState φa]ₛca * b) = 0 := by
   simp only [superCommuteF_ofCrAnState_ofCrAnState, instCommGroup.eq_1, Algebra.smul_mul_assoc]
   rw [mul_sub, sub_mul, map_sub, ← smul_mul_assoc, ← mul_assoc, ← mul_assoc,
-    normalOrder_swap_create_annihlate φc φa hφc hφa]
+    normalOrderF_swap_create_annihlate φc φa hφc hφa]
   simp
 
-lemma normalOrder_superCommuteF_annihilate_create (φc φa : 𝓕.CrAnStates)
+lemma normalOrderF_superCommuteF_annihilate_create (φc φa : 𝓕.CrAnStates)
     (hφc : 𝓕 |>ᶜ φc = CreateAnnihilate.create) (hφa : 𝓕 |>ᶜ φa = CreateAnnihilate.annihilate)
     (a b : 𝓕.CrAnAlgebra) :
     𝓝ᶠ(a * [ofCrAnState φa, ofCrAnState φc]ₛca * b) = 0 := by
   rw [superCommuteF_ofCrAnState_ofCrAnState_symm]
   simp only [instCommGroup.eq_1, neg_smul, mul_neg, Algebra.mul_smul_comm, neg_mul,
     Algebra.smul_mul_assoc, map_neg, map_smul, neg_eq_zero, smul_eq_zero]
-  exact Or.inr (normalOrder_superCommuteF_create_annihilate φc φa hφc hφa ..)
+  exact Or.inr (normalOrderF_superCommuteF_create_annihilate φc φa hφc hφa ..)
 
-lemma normalOrder_swap_crPart_anPart (φ φ' : 𝓕.States) (a b : CrAnAlgebra 𝓕) :
+lemma normalOrderF_swap_crPart_anPart (φ φ' : 𝓕.States) (a b : CrAnAlgebra 𝓕) :
     𝓝ᶠ(a * (crPart φ) * (anPart φ') * b) =
     𝓢(𝓕 |>ₛ φ, 𝓕 |>ₛ φ') •
     𝓝ᶠ(a * (anPart φ') * (crPart φ) * b) := by
@@ -190,22 +190,22 @@ lemma normalOrder_swap_crPart_anPart (φ φ' : 𝓕.States) (a b : CrAnAlgebra �
   | .outAsymp φ, _ => simp
   | .position φ, .position φ' =>
     simp only [crPart_position, anPart_position, instCommGroup.eq_1]
-    rw [normalOrder_swap_create_annihlate]
+    rw [normalOrderF_swap_create_annihlate]
     simp only [instCommGroup.eq_1, crAnStatistics, Function.comp_apply, crAnStatesToStates_prod]
     rfl; rfl
   | .inAsymp φ, .outAsymp φ' =>
     simp only [crPart_negAsymp, anPart_posAsymp, instCommGroup.eq_1]
-    rw [normalOrder_swap_create_annihlate]
+    rw [normalOrderF_swap_create_annihlate]
     simp only [instCommGroup.eq_1, crAnStatistics, Function.comp_apply, crAnStatesToStates_prod]
     rfl; rfl
   | .inAsymp φ, .position φ' =>
     simp only [crPart_negAsymp, anPart_position, instCommGroup.eq_1]
-    rw [normalOrder_swap_create_annihlate]
+    rw [normalOrderF_swap_create_annihlate]
     simp only [instCommGroup.eq_1, crAnStatistics, Function.comp_apply, crAnStatesToStates_prod]
     rfl; rfl
   | .position φ, .outAsymp φ' =>
     simp only [crPart_position, anPart_posAsymp, instCommGroup.eq_1]
-    rw [normalOrder_swap_create_annihlate]
+    rw [normalOrderF_swap_create_annihlate]
     simp only [instCommGroup.eq_1, crAnStatistics, Function.comp_apply, crAnStatesToStates_prod]
     rfl; rfl
 
@@ -217,13 +217,13 @@ Using the results from above.
 
 -/
 
-lemma normalOrder_swap_anPart_crPart (φ φ' : 𝓕.States) (a b : CrAnAlgebra 𝓕) :
+lemma normalOrderF_swap_anPart_crPart (φ φ' : 𝓕.States) (a b : CrAnAlgebra 𝓕) :
     𝓝ᶠ(a * (anPart φ) * (crPart φ') * b) =
     𝓢(𝓕 |>ₛ φ, 𝓕 |>ₛ φ') • 𝓝ᶠ(a * (crPart φ') *
       (anPart φ) * b) := by
-  simp [normalOrder_swap_crPart_anPart, smul_smul]
+  simp [normalOrderF_swap_crPart_anPart, smul_smul]
 
-lemma normalOrder_superCommuteF_crPart_anPart (φ φ' : 𝓕.States) (a b : CrAnAlgebra 𝓕) :
+lemma normalOrderF_superCommuteF_crPart_anPart (φ φ' : 𝓕.States) (a b : CrAnAlgebra 𝓕) :
     𝓝ᶠ(a * superCommuteF
       (crPart φ) (anPart φ') * b) = 0 := by
   match φ, φ' with
@@ -231,18 +231,18 @@ lemma normalOrder_superCommuteF_crPart_anPart (φ φ' : 𝓕.States) (a b : CrAn
   | .outAsymp φ', _ => simp
   | .position φ, .position φ' =>
     rw [crPart_position, anPart_position]
-    exact normalOrder_superCommuteF_create_annihilate _ _ rfl rfl ..
+    exact normalOrderF_superCommuteF_create_annihilate _ _ rfl rfl ..
   | .inAsymp φ, .outAsymp φ' =>
     rw [crPart_negAsymp, anPart_posAsymp]
-    exact normalOrder_superCommuteF_create_annihilate _ _ rfl rfl ..
+    exact normalOrderF_superCommuteF_create_annihilate _ _ rfl rfl ..
   | .inAsymp φ, .position φ' =>
     rw [crPart_negAsymp, anPart_position]
-    exact normalOrder_superCommuteF_create_annihilate _ _ rfl rfl ..
+    exact normalOrderF_superCommuteF_create_annihilate _ _ rfl rfl ..
   | .position φ, .outAsymp φ' =>
     rw [crPart_position, anPart_posAsymp]
-    exact normalOrder_superCommuteF_create_annihilate _ _ rfl rfl ..
+    exact normalOrderF_superCommuteF_create_annihilate _ _ rfl rfl ..
 
-lemma normalOrder_superCommuteF_anPart_crPart (φ φ' : 𝓕.States) (a b : CrAnAlgebra 𝓕) :
+lemma normalOrderF_superCommuteF_anPart_crPart (φ φ' : 𝓕.States) (a b : CrAnAlgebra 𝓕) :
     𝓝ᶠ(a * superCommuteF
     (anPart φ) (crPart φ') * b) = 0 := by
   match φ, φ' with
@@ -250,16 +250,16 @@ lemma normalOrder_superCommuteF_anPart_crPart (φ φ' : 𝓕.States) (a b : CrAn
   | _, .outAsymp φ' => simp
   | .position φ, .position φ' =>
     rw [anPart_position, crPart_position]
-    exact normalOrder_superCommuteF_annihilate_create _ _ rfl rfl ..
+    exact normalOrderF_superCommuteF_annihilate_create _ _ rfl rfl ..
   | .outAsymp φ', .inAsymp φ =>
     simp only [anPart_posAsymp, crPart_negAsymp]
-    exact normalOrder_superCommuteF_annihilate_create _ _ rfl rfl ..
+    exact normalOrderF_superCommuteF_annihilate_create _ _ rfl rfl ..
   | .position φ', .inAsymp φ =>
     simp only [anPart_position, crPart_negAsymp]
-    exact normalOrder_superCommuteF_annihilate_create _ _ rfl rfl ..
+    exact normalOrderF_superCommuteF_annihilate_create _ _ rfl rfl ..
   | .outAsymp φ, .position φ' =>
     simp only [anPart_posAsymp, crPart_position]
-    exact normalOrder_superCommuteF_annihilate_create _ _ rfl rfl ..
+    exact normalOrderF_superCommuteF_annihilate_create _ _ rfl rfl ..
 
 /-!
 
@@ -268,44 +268,44 @@ lemma normalOrder_superCommuteF_anPart_crPart (φ φ' : 𝓕.States) (a b : CrAn
 -/
 
 @[simp]
-lemma normalOrder_crPart_mul_crPart (φ φ' : 𝓕.States) :
+lemma normalOrderF_crPart_mul_crPart (φ φ' : 𝓕.States) :
     𝓝ᶠ(crPart φ * crPart φ') =
     crPart φ * crPart φ' := by
-  rw [normalOrder_crPart_mul]
+  rw [normalOrderF_crPart_mul]
   conv_lhs => rw [← mul_one (crPart φ')]
-  rw [normalOrder_crPart_mul, normalOrder_one]
+  rw [normalOrderF_crPart_mul, normalOrderF_one]
   simp
 
 @[simp]
-lemma normalOrder_anPart_mul_anPart (φ φ' : 𝓕.States) :
+lemma normalOrderF_anPart_mul_anPart (φ φ' : 𝓕.States) :
     𝓝ᶠ(anPart φ * anPart φ') =
     anPart φ * anPart φ' := by
-  rw [normalOrder_mul_anPart]
+  rw [normalOrderF_mul_anPart]
   conv_lhs => rw [← one_mul (anPart φ)]
-  rw [normalOrder_mul_anPart, normalOrder_one]
+  rw [normalOrderF_mul_anPart, normalOrderF_one]
   simp
 
 @[simp]
-lemma normalOrder_crPart_mul_anPart (φ φ' : 𝓕.States) :
+lemma normalOrderF_crPart_mul_anPart (φ φ' : 𝓕.States) :
     𝓝ᶠ(crPart φ * anPart φ') =
     crPart φ * anPart φ' := by
-  rw [normalOrder_crPart_mul]
+  rw [normalOrderF_crPart_mul]
   conv_lhs => rw [← one_mul (anPart φ')]
-  rw [normalOrder_mul_anPart, normalOrder_one]
+  rw [normalOrderF_mul_anPart, normalOrderF_one]
   simp
 
 @[simp]
-lemma normalOrder_anPart_mul_crPart (φ φ' : 𝓕.States) :
+lemma normalOrderF_anPart_mul_crPart (φ φ' : 𝓕.States) :
     𝓝ᶠ(anPart φ * crPart φ') =
     𝓢(𝓕 |>ₛ φ, 𝓕 |>ₛ φ') •
     (crPart φ' * anPart φ) := by
   conv_lhs => rw [← one_mul (anPart φ * crPart φ')]
   conv_lhs => rw [← mul_one (1 * (anPart φ *
     crPart φ'))]
-  rw [← mul_assoc, normalOrder_swap_anPart_crPart]
+  rw [← mul_assoc, normalOrderF_swap_anPart_crPart]
   simp
 
-lemma normalOrder_ofState_mul_ofState (φ φ' : 𝓕.States) :
+lemma normalOrderF_ofState_mul_ofState (φ φ' : 𝓕.States) :
     𝓝ᶠ(ofState φ * ofState φ') =
     crPart φ * crPart φ' +
     𝓢(𝓕 |>ₛ φ, 𝓕 |>ₛ φ') •
@@ -313,8 +313,8 @@ lemma normalOrder_ofState_mul_ofState (φ φ' : 𝓕.States) :
     crPart φ * anPart φ' +
     anPart φ * anPart φ' := by
   rw [ofState_eq_crPart_add_anPart, ofState_eq_crPart_add_anPart, mul_add, add_mul, add_mul]
-  simp only [map_add, normalOrder_crPart_mul_crPart, normalOrder_anPart_mul_crPart,
-    instCommGroup.eq_1, normalOrder_crPart_mul_anPart, normalOrder_anPart_mul_anPart]
+  simp only [map_add, normalOrderF_crPart_mul_crPart, normalOrderF_anPart_mul_crPart,
+    instCommGroup.eq_1, normalOrderF_crPart_mul_anPart, normalOrderF_anPart_mul_anPart]
   abel
 
 /-!
@@ -325,7 +325,7 @@ lemma normalOrder_ofState_mul_ofState (φ φ' : 𝓕.States) :
 
 TODO "Split the following two lemmas up into smaller parts."
 
-lemma normalOrder_superCommuteF_ofCrAnList_create_create_ofCrAnList
+lemma normalOrderF_superCommuteF_ofCrAnList_create_create_ofCrAnList
     (φc φc' : 𝓕.CrAnStates) (hφc : 𝓕 |>ᶜ φc = CreateAnnihilate.create)
     (hφc' : 𝓕 |>ᶜ φc' = CreateAnnihilate.create) (φs φs' : List 𝓕.CrAnStates) :
     (𝓝ᶠ(ofCrAnList φs * [ofCrAnState φc, ofCrAnState φc']ₛca * ofCrAnList φs')) =
@@ -339,7 +339,7 @@ lemma normalOrder_superCommuteF_ofCrAnList_create_create_ofCrAnList
       ← ofCrAnList_append]
   conv_lhs =>
     lhs
-    rw [normalOrder_ofCrAnList, normalOrderList_eq_createFilter_append_annihilateFilter]
+    rw [normalOrderF_ofCrAnList, normalOrderList_eq_createFilter_append_annihilateFilter]
     rw [createFilter_append, createFilter_append, createFilter_append,
       createFilter_singleton_create _ hφc, createFilter_singleton_create _ hφc']
     rw [annihilateFilter_append, annihilateFilter_append, annihilateFilter_append,
@@ -358,7 +358,7 @@ lemma normalOrder_superCommuteF_ofCrAnList_create_create_ofCrAnList
     rhs
     rw [map_smul]
     rhs
-    rw [normalOrder_ofCrAnList, normalOrderList_eq_createFilter_append_annihilateFilter]
+    rw [normalOrderF_ofCrAnList, normalOrderList_eq_createFilter_append_annihilateFilter]
     rw [createFilter_append, createFilter_append, createFilter_append,
       createFilter_singleton_create _ hφc, createFilter_singleton_create _ hφc']
     rw [annihilateFilter_append, annihilateFilter_append, annihilateFilter_append,
@@ -384,7 +384,7 @@ lemma normalOrder_superCommuteF_ofCrAnList_create_create_ofCrAnList
     ofCrAnList_singleton]
   rw [ofCrAnList_append, ofCrAnList_singleton, ofCrAnList_singleton, smul_mul_assoc]
 
-lemma normalOrder_superCommuteF_ofCrAnList_annihilate_annihilate_ofCrAnList
+lemma normalOrderF_superCommuteF_ofCrAnList_annihilate_annihilate_ofCrAnList
     (φa φa' : 𝓕.CrAnStates)
     (hφa : 𝓕 |>ᶜ φa = CreateAnnihilate.annihilate)
     (hφa' : 𝓕 |>ᶜ φa' = CreateAnnihilate.annihilate)
@@ -401,7 +401,7 @@ lemma normalOrder_superCommuteF_ofCrAnList_annihilate_annihilate_ofCrAnList
       ← ofCrAnList_append]
   conv_lhs =>
     lhs
-    rw [normalOrder_ofCrAnList, normalOrderList_eq_createFilter_append_annihilateFilter]
+    rw [normalOrderF_ofCrAnList, normalOrderList_eq_createFilter_append_annihilateFilter]
     rw [createFilter_append, createFilter_append, createFilter_append,
       createFilter_singleton_annihilate _ hφa, createFilter_singleton_annihilate _ hφa']
     rw [annihilateFilter_append, annihilateFilter_append, annihilateFilter_append,
@@ -421,7 +421,7 @@ lemma normalOrder_superCommuteF_ofCrAnList_annihilate_annihilate_ofCrAnList
     rhs
     rw [map_smul]
     rhs
-    rw [normalOrder_ofCrAnList, normalOrderList_eq_createFilter_append_annihilateFilter]
+    rw [normalOrderF_ofCrAnList, normalOrderList_eq_createFilter_append_annihilateFilter]
     rw [createFilter_append, createFilter_append, createFilter_append,
       createFilter_singleton_annihilate _ hφa, createFilter_singleton_annihilate _ hφa']
     rw [annihilateFilter_append, annihilateFilter_append, annihilateFilter_append,
@@ -458,14 +458,14 @@ lemma normalOrder_superCommuteF_ofCrAnList_annihilate_annihilate_ofCrAnList
 
 -/
 
-lemma ofCrAnList_superCommuteF_normalOrder_ofCrAnList (φs φs' : List 𝓕.CrAnStates) :
+lemma ofCrAnList_superCommuteF_normalOrderF_ofCrAnList (φs φs' : List 𝓕.CrAnStates) :
     [ofCrAnList φs, 𝓝ᶠ(ofCrAnList φs')]ₛca =
     ofCrAnList φs * 𝓝ᶠ(ofCrAnList φs') -
     𝓢(𝓕 |>ₛ φs, 𝓕 |>ₛ φs') • 𝓝ᶠ(ofCrAnList φs') * ofCrAnList φs := by
-  simp [normalOrder_ofCrAnList, map_smul, superCommuteF_ofCrAnList_ofCrAnList, ofCrAnList_append,
+  simp [normalOrderF_ofCrAnList, map_smul, superCommuteF_ofCrAnList_ofCrAnList, ofCrAnList_append,
     smul_sub, smul_smul, mul_comm]
 
-lemma ofCrAnList_superCommuteF_normalOrder_ofStateList (φs : List 𝓕.CrAnStates)
+lemma ofCrAnList_superCommuteF_normalOrderF_ofStateList (φs : List 𝓕.CrAnStates)
     (φs' : List 𝓕.States) : [ofCrAnList φs, 𝓝ᶠ(ofStateList φs')]ₛca =
     ofCrAnList φs * 𝓝ᶠ(ofStateList φs') -
     𝓢(𝓕 |>ₛ φs, 𝓕 |>ₛ φs') • 𝓝ᶠ(ofStateList φs') * ofCrAnList φs := by
@@ -473,7 +473,7 @@ lemma ofCrAnList_superCommuteF_normalOrder_ofStateList (φs : List 𝓕.CrAnStat
     ← Finset.sum_sub_distrib, map_sum]
   congr
   funext n
-  rw [ofCrAnList_superCommuteF_normalOrder_ofCrAnList,
+  rw [ofCrAnList_superCommuteF_normalOrderF_ofCrAnList,
     CrAnSection.statistics_eq_state_statistics]
 
 /-!
@@ -482,29 +482,29 @@ lemma ofCrAnList_superCommuteF_normalOrder_ofStateList (φs : List 𝓕.CrAnStat
 
 -/
 
-lemma ofCrAnList_mul_normalOrder_ofStateList_eq_superCommuteF (φs : List 𝓕.CrAnStates)
+lemma ofCrAnList_mul_normalOrderF_ofStateList_eq_superCommuteF (φs : List 𝓕.CrAnStates)
     (φs' : List 𝓕.States) :
     ofCrAnList φs * 𝓝ᶠ(ofStateList φs') =
     𝓢(𝓕 |>ₛ φs, 𝓕 |>ₛ φs') • 𝓝ᶠ(ofStateList φs') * ofCrAnList φs
     + [ofCrAnList φs, 𝓝ᶠ(ofStateList φs')]ₛca := by
-  simp [ofCrAnList_superCommuteF_normalOrder_ofStateList]
+  simp [ofCrAnList_superCommuteF_normalOrderF_ofStateList]
 
-lemma ofCrAnState_mul_normalOrder_ofStateList_eq_superCommuteF (φ : 𝓕.CrAnStates)
+lemma ofCrAnState_mul_normalOrderF_ofStateList_eq_superCommuteF (φ : 𝓕.CrAnStates)
     (φs' : List 𝓕.States) : ofCrAnState φ * 𝓝ᶠ(ofStateList φs') =
     𝓢(𝓕 |>ₛ φ, 𝓕 |>ₛ φs') • 𝓝ᶠ(ofStateList φs') * ofCrAnState φ
     + [ofCrAnState φ, 𝓝ᶠ(ofStateList φs')]ₛca := by
-  simp [← ofCrAnList_singleton, ofCrAnList_mul_normalOrder_ofStateList_eq_superCommuteF]
+  simp [← ofCrAnList_singleton, ofCrAnList_mul_normalOrderF_ofStateList_eq_superCommuteF]
 
-lemma anPart_mul_normalOrder_ofStateList_eq_superCommuteF (φ : 𝓕.States)
+lemma anPart_mul_normalOrderF_ofStateList_eq_superCommuteF (φ : 𝓕.States)
     (φs' : List 𝓕.States) :
     anPart φ * 𝓝ᶠ(ofStateList φs') =
     𝓢(𝓕 |>ₛ φ, 𝓕 |>ₛ φs') • 𝓝ᶠ(ofStateList φs' * anPart φ)
     + [anPart φ, 𝓝ᶠ(ofStateList φs')]ₛca := by
-  rw [normalOrder_mul_anPart]
+  rw [normalOrderF_mul_anPart]
   match φ with
   | .inAsymp φ => simp
-  | .position φ => simp [ofCrAnState_mul_normalOrder_ofStateList_eq_superCommuteF, crAnStatistics]
-  | .outAsymp φ => simp [ofCrAnState_mul_normalOrder_ofStateList_eq_superCommuteF, crAnStatistics]
+  | .position φ => simp [ofCrAnState_mul_normalOrderF_ofStateList_eq_superCommuteF, crAnStatistics]
+  | .outAsymp φ => simp [ofCrAnState_mul_normalOrderF_ofStateList_eq_superCommuteF, crAnStatistics]
 
 end
 
