HepLean/PerturbationTheory/Algebras/FieldOpAlgebra/NormalOrder.lean
@@ -24,53 +24,53 @@ variable {𝓕 : FieldSpecification}
 ## Normal order on super-commutators.
 
 The main result of this is
-`ι_normalOrder_superCommuteF_eq_zero_mul`
+`ι_normalOrderF_superCommuteF_eq_zero_mul`
 which states that applying `ι` to the normal order of something containing a super-commutator
 is zero.
 
 -/
 
-lemma ι_normalOrder_superCommuteF_ofCrAnList_ofCrAnList_eq_zero
+lemma ι_normalOrderF_superCommuteF_ofCrAnList_ofCrAnList_eq_zero
     (φa φa' : 𝓕.CrAnStates) (φs φs' : List 𝓕.CrAnStates) :
     ι 𝓝ᶠ(ofCrAnList φs * [ofCrAnState φa, ofCrAnState φa']ₛca * ofCrAnList φs') = 0 := by
   rcases CreateAnnihilate.eq_create_or_annihilate (𝓕 |>ᶜ φa) with hφa | hφa
   <;> rcases CreateAnnihilate.eq_create_or_annihilate (𝓕 |>ᶜ φa') with hφa' | hφa'
-  · rw [normalOrder_superCommuteF_ofCrAnList_create_create_ofCrAnList φa φa' hφa hφa' φs φs']
+  · rw [normalOrderF_superCommuteF_ofCrAnList_create_create_ofCrAnList φa φa' hφa hφa' φs φs']
     rw [map_smul, map_mul, map_mul, map_mul, ι_superCommuteF_of_create_create φa φa' hφa hφa']
     simp
-  · rw [normalOrder_superCommuteF_create_annihilate φa φa' hφa hφa' (ofCrAnList φs)
+  · rw [normalOrderF_superCommuteF_create_annihilate φa φa' hφa hφa' (ofCrAnList φs)
       (ofCrAnList φs')]
     simp
-  · rw [normalOrder_superCommuteF_annihilate_create φa' φa hφa' hφa (ofCrAnList φs)
+  · rw [normalOrderF_superCommuteF_annihilate_create φa' φa hφa' hφa (ofCrAnList φs)
       (ofCrAnList φs')]
     simp
-  · rw [normalOrder_superCommuteF_ofCrAnList_annihilate_annihilate_ofCrAnList φa φa' hφa hφa' φs φs']
+  · rw [normalOrderF_superCommuteF_ofCrAnList_annihilate_annihilate_ofCrAnList φa φa' hφa hφa' φs φs']
     rw [map_smul, map_mul, map_mul, map_mul,
       ι_superCommuteF_of_annihilate_annihilate φa φa' hφa hφa']
     simp
 
-lemma ι_normalOrder_superCommuteF_ofCrAnList_eq_zero
+lemma ι_normalOrderF_superCommuteF_ofCrAnList_eq_zero
     (φa φa' : 𝓕.CrAnStates) (φs : List 𝓕.CrAnStates)
     (a : 𝓕.CrAnAlgebra) : ι 𝓝ᶠ(ofCrAnList φs * [ofCrAnState φa, ofCrAnState φa']ₛca * a) = 0 := by
-  have hf : ι.toLinearMap ∘ₗ normalOrder ∘ₗ
+  have hf : ι.toLinearMap ∘ₗ normalOrderF ∘ₗ
       mulLinearMap (ofCrAnList φs * [ofCrAnState φa, ofCrAnState φa']ₛca) = 0 := by
     apply ofCrAnListBasis.ext
     intro l
     simp only [CrAnAlgebra.ofListBasis_eq_ofList, LinearMap.coe_comp, Function.comp_apply,
       AlgHom.toLinearMap_apply, LinearMap.zero_apply]
-    exact ι_normalOrder_superCommuteF_ofCrAnList_ofCrAnList_eq_zero φa φa' φs l
-  change (ι.toLinearMap ∘ₗ normalOrder ∘ₗ
+    exact ι_normalOrderF_superCommuteF_ofCrAnList_ofCrAnList_eq_zero φa φa' φs l
+  change (ι.toLinearMap ∘ₗ normalOrderF ∘ₗ
     mulLinearMap ((ofCrAnList φs * [ofCrAnState φa, ofCrAnState φa']ₛca))) a = 0
   rw [hf]
   simp
 
-lemma ι_normalOrder_superCommuteF_ofCrAnState_eq_zero_mul (φa φa' : 𝓕.CrAnStates)
+lemma ι_normalOrderF_superCommuteF_ofCrAnState_eq_zero_mul (φa φa' : 𝓕.CrAnStates)
     (a b : 𝓕.CrAnAlgebra) :
     ι 𝓝ᶠ(a * [ofCrAnState φa, ofCrAnState φa']ₛca * b) = 0 := by
   rw [mul_assoc]
-  change (ι.toLinearMap ∘ₗ normalOrder ∘ₗ mulLinearMap.flip
+  change (ι.toLinearMap ∘ₗ normalOrderF ∘ₗ mulLinearMap.flip
     ([ofCrAnState φa, ofCrAnState φa']ₛca * b)) a = 0
-  have hf : ι.toLinearMap ∘ₗ normalOrder ∘ₗ mulLinearMap.flip
+  have hf : ι.toLinearMap ∘ₗ normalOrderF ∘ₗ mulLinearMap.flip
       ([ofCrAnState φa, ofCrAnState φa']ₛca * b) = 0 := by
     apply ofCrAnListBasis.ext
     intro l
@@ -78,11 +78,11 @@ lemma ι_normalOrder_superCommuteF_ofCrAnState_eq_zero_mul (φa φa' : 𝓕.CrAn
       Function.comp_apply, LinearMap.flip_apply, LinearMap.coe_mk, AddHom.coe_mk,
       AlgHom.toLinearMap_apply, LinearMap.zero_apply]
     rw [← mul_assoc]
-    exact ι_normalOrder_superCommuteF_ofCrAnList_eq_zero φa φa' _ _
+    exact ι_normalOrderF_superCommuteF_ofCrAnList_eq_zero φa φa' _ _
   rw [hf]
   simp
 
-lemma ι_normalOrder_superCommuteF_ofCrAnState_ofCrAnList_eq_zero_mul (φa : 𝓕.CrAnStates)
+lemma ι_normalOrderF_superCommuteF_ofCrAnState_ofCrAnList_eq_zero_mul (φa : 𝓕.CrAnStates)
     (φs : List 𝓕.CrAnStates)
     (a b : 𝓕.CrAnAlgebra) :
     ι 𝓝ᶠ(a * [ofCrAnState φa, ofCrAnList φs]ₛca * b) = 0 := by
@@ -93,18 +93,18 @@ lemma ι_normalOrder_superCommuteF_ofCrAnState_ofCrAnList_eq_zero_mul (φa : �
   intro n
   rw [← mul_assoc, ← mul_assoc]
   rw [mul_assoc _ _ b, ofCrAnList_singleton]
-  rw [ι_normalOrder_superCommuteF_ofCrAnState_eq_zero_mul]
+  rw [ι_normalOrderF_superCommuteF_ofCrAnState_eq_zero_mul]
 
-lemma ι_normalOrder_superCommuteF_ofCrAnList_ofCrAnState_eq_zero_mul (φa : 𝓕.CrAnStates)
+lemma ι_normalOrderF_superCommuteF_ofCrAnList_ofCrAnState_eq_zero_mul (φa : 𝓕.CrAnStates)
     (φs : List 𝓕.CrAnStates) (a b : 𝓕.CrAnAlgebra) :
     ι 𝓝ᶠ(a * [ofCrAnList φs, ofCrAnState φa]ₛca * b) = 0 := by
   rw [← ofCrAnList_singleton, superCommuteF_ofCrAnList_ofCrAnList_symm, ofCrAnList_singleton]
   simp only [FieldStatistic.instCommGroup.eq_1, FieldStatistic.ofList_singleton, mul_neg,
     Algebra.mul_smul_comm, neg_mul, Algebra.smul_mul_assoc, map_neg, map_smul]
-  rw [ι_normalOrder_superCommuteF_ofCrAnState_ofCrAnList_eq_zero_mul]
+  rw [ι_normalOrderF_superCommuteF_ofCrAnState_ofCrAnList_eq_zero_mul]
   simp
 
-lemma ι_normalOrder_superCommuteF_ofCrAnList_ofCrAnList_eq_zero_mul
+lemma ι_normalOrderF_superCommuteF_ofCrAnList_ofCrAnList_eq_zero_mul
     (φs φs' : List 𝓕.CrAnStates) (a b : 𝓕.CrAnAlgebra) :
     ι 𝓝ᶠ(a * [ofCrAnList φs, ofCrAnList φs']ₛca * b) = 0 := by
   rw [superCommuteF_ofCrAnList_ofCrAnList_eq_sum, Finset.mul_sum, Finset.sum_mul]
@@ -113,63 +113,63 @@ lemma ι_normalOrder_superCommuteF_ofCrAnList_ofCrAnList_eq_zero_mul
   intro n
   rw [← mul_assoc, ← mul_assoc]
   rw [mul_assoc _ _ b]
-  rw [ι_normalOrder_superCommuteF_ofCrAnList_ofCrAnState_eq_zero_mul]
+  rw [ι_normalOrderF_superCommuteF_ofCrAnList_ofCrAnState_eq_zero_mul]
 
-lemma ι_normalOrder_superCommuteF_ofCrAnList_eq_zero_mul
+lemma ι_normalOrderF_superCommuteF_ofCrAnList_eq_zero_mul
     (φs : List 𝓕.CrAnStates)
     (a b c : 𝓕.CrAnAlgebra) :
     ι 𝓝ᶠ(a * [ofCrAnList φs, c]ₛca * b) = 0 := by
-  change (ι.toLinearMap ∘ₗ normalOrder ∘ₗ
+  change (ι.toLinearMap ∘ₗ normalOrderF ∘ₗ
     mulLinearMap.flip b ∘ₗ mulLinearMap a ∘ₗ superCommuteF (ofCrAnList φs)) c = 0
-  have hf : (ι.toLinearMap ∘ₗ normalOrder ∘ₗ
+  have hf : (ι.toLinearMap ∘ₗ normalOrderF ∘ₗ
     mulLinearMap.flip b ∘ₗ mulLinearMap a ∘ₗ superCommuteF (ofCrAnList φs)) = 0 := by
     apply ofCrAnListBasis.ext
     intro φs'
     simp only [mulLinearMap, LinearMap.coe_mk, AddHom.coe_mk, CrAnAlgebra.ofListBasis_eq_ofList,
       LinearMap.coe_comp, Function.comp_apply, LinearMap.flip_apply, AlgHom.toLinearMap_apply,
       LinearMap.zero_apply]
-    rw [ι_normalOrder_superCommuteF_ofCrAnList_ofCrAnList_eq_zero_mul]
+    rw [ι_normalOrderF_superCommuteF_ofCrAnList_ofCrAnList_eq_zero_mul]
   rw [hf]
   simp
 
 @[simp]
-lemma ι_normalOrder_superCommuteF_eq_zero_mul
+lemma ι_normalOrderF_superCommuteF_eq_zero_mul
     (a b c d : 𝓕.CrAnAlgebra) : ι 𝓝ᶠ(a * [d, c]ₛca * b) = 0 := by
-  change (ι.toLinearMap ∘ₗ normalOrder ∘ₗ
+  change (ι.toLinearMap ∘ₗ normalOrderF ∘ₗ
     mulLinearMap.flip b ∘ₗ mulLinearMap a ∘ₗ superCommuteF.flip c) d = 0
-  have hf : (ι.toLinearMap ∘ₗ normalOrder ∘ₗ
+  have hf : (ι.toLinearMap ∘ₗ normalOrderF ∘ₗ
     mulLinearMap.flip b ∘ₗ mulLinearMap a ∘ₗ superCommuteF.flip c) = 0 := by
     apply ofCrAnListBasis.ext
     intro φs
     simp only [mulLinearMap, LinearMap.coe_mk, AddHom.coe_mk, CrAnAlgebra.ofListBasis_eq_ofList,
       LinearMap.coe_comp, Function.comp_apply, LinearMap.flip_apply, AlgHom.toLinearMap_apply,
       LinearMap.zero_apply]
-    rw [ι_normalOrder_superCommuteF_ofCrAnList_eq_zero_mul]
+    rw [ι_normalOrderF_superCommuteF_ofCrAnList_eq_zero_mul]
   rw [hf]
   simp
 
 @[simp]
 lemma ι_normalOrder_superCommuteF_eq_zero_mul_right (b c d : 𝓕.CrAnAlgebra) :
     ι 𝓝ᶠ([d, c]ₛca * b) = 0 := by
-  rw [← ι_normalOrder_superCommuteF_eq_zero_mul 1 b c d]
+  rw [← ι_normalOrderF_superCommuteF_eq_zero_mul 1 b c d]
   simp
 
 @[simp]
-lemma ι_normalOrder_superCommuteF_eq_zero_mul_left (a c d : 𝓕.CrAnAlgebra) :
+lemma ι_normalOrderF_superCommuteF_eq_zero_mul_left (a c d : 𝓕.CrAnAlgebra) :
     ι 𝓝ᶠ(a * [d, c]ₛca) = 0 := by
-  rw [← ι_normalOrder_superCommuteF_eq_zero_mul a 1 c d]
+  rw [← ι_normalOrderF_superCommuteF_eq_zero_mul a 1 c d]
   simp
 
 @[simp]
-lemma ι_normalOrder_superCommuteF_eq_zero_mul_mul_right (a b1 b2 c d: 𝓕.CrAnAlgebra) :
+lemma ι_normalOrderF_superCommuteF_eq_zero_mul_mul_right (a b1 b2 c d: 𝓕.CrAnAlgebra) :
     ι 𝓝ᶠ(a * [d, c]ₛca * b1 * b2) = 0 := by
-  rw [← ι_normalOrder_superCommuteF_eq_zero_mul a (b1 * b2) c d]
+  rw [← ι_normalOrderF_superCommuteF_eq_zero_mul a (b1 * b2) c d]
   congr 2
   noncomm_ring
 
 @[simp]
-lemma ι_normalOrder_superCommuteF_eq_zero (c d : 𝓕.CrAnAlgebra) : ι 𝓝ᶠ([d, c]ₛca) = 0 := by
-  rw [← ι_normalOrder_superCommuteF_eq_zero_mul 1 1 c d]
+lemma ι_normalOrderF_superCommuteF_eq_zero (c d : 𝓕.CrAnAlgebra) : ι 𝓝ᶠ([d, c]ₛca) = 0 := by
+  rw [← ι_normalOrderF_superCommuteF_eq_zero_mul 1 1 c d]
   simp
 
 /-!
@@ -178,7 +178,7 @@ lemma ι_normalOrder_superCommuteF_eq_zero (c d : 𝓕.CrAnAlgebra) : ι 𝓝ᶠ
 
 -/
 
-lemma ι_normalOrder_zero_of_mem_ideal (a : 𝓕.CrAnAlgebra)
+lemma ι_normalOrderF_zero_of_mem_ideal (a : 𝓕.CrAnAlgebra)
     (h : a ∈ TwoSidedIdeal.span 𝓕.fieldOpIdealSet) : ι 𝓝ᶠ(a) = 0 := by
   rw [TwoSidedIdeal.mem_span_iff_mem_addSubgroup_closure] at h
   let p {k : Set 𝓕.CrAnAlgebra} (a : CrAnAlgebra 𝓕) (h : a ∈ AddSubgroup.closure k) := ι 𝓝ᶠ(a) = 0
@@ -210,16 +210,16 @@ lemma ι_normalOrder_zero_of_mem_ideal (a : 𝓕.CrAnAlgebra)
   · intro x hx
     simp [p]
 
-lemma ι_normalOrder_eq_of_equiv (a b : 𝓕.CrAnAlgebra) (h : a ≈ b) :
+lemma ι_normalOrderF_eq_of_equiv (a b : 𝓕.CrAnAlgebra) (h : a ≈ b) :
     ι 𝓝ᶠ(a) = ι 𝓝ᶠ(b) := by
   rw [equiv_iff_sub_mem_ideal] at h
   rw [LinearMap.sub_mem_ker_iff.mp]
   simp only [LinearMap.mem_ker, ← map_sub]
-  exact ι_normalOrder_zero_of_mem_ideal (a - b) h
+  exact ι_normalOrderF_zero_of_mem_ideal (a - b) h
 
 /-- Normal ordering on `FieldOpAlgebra`. -/
 noncomputable def normalOrder : FieldOpAlgebra 𝓕 →ₗ[ℂ] FieldOpAlgebra 𝓕 where
-  toFun := Quotient.lift (ι.toLinearMap ∘ₗ CrAnAlgebra.normalOrder) ι_normalOrder_eq_of_equiv
+  toFun := Quotient.lift (ι.toLinearMap ∘ₗ normalOrderF) ι_normalOrderF_eq_of_equiv
   map_add' x y := by
     obtain ⟨x, rfl⟩ := ι_surjective x
     obtain ⟨y, rfl⟩ := ι_surjective y
